@prefix : <http://linked.data.gov.au/def/borehole/> .
@prefix dc: <http://purl.org/dc/elements/1.1/> .
@prefix dct: <http://purl.org/dc/terms/> .
@prefix geo: <http://www.opengis.net/ont/geosparql#> .
@prefix gsq: <http://linked.data.gov.au/def/gsq> .
@prefix owl: <http://www.w3.org/2002/07/owl#> .
@prefix rdf: <http://www.w3.org/1999/02/22-rdf-syntax-ns#> .
@prefix sdo: <https://schema.org/> .
@prefix xml: <http://www.w3.org/XML/1998/namespace> .
@prefix xsd: <http://www.w3.org/2001/XMLSchema#> .
@prefix asgs: <http://linked.data.gov.au/def/asgs#> .
@prefix geox: <http://linked.data.gov.au/def/geox/> .
@prefix loci: <http://linked.data.gov.au/def/loci/> .
@prefix prov: <http://www.w3.org/ns/prov#> .
@prefix qudt: <http://qudt.org/schema/qudt/> .
@prefix rdfs: <http://www.w3.org/2000/01/rdf-schema#> .
@prefix skos: <http://www.w3.org/2004/02/skos/core#> .
@prefix time: <http://www.w3.org/2006/time#> .
@base <http://linked.data.gov.au/def/borehole> .

<http://linked.data.gov.au/def/borehole> rdf:type owl:Ontology ;
                                          dct:modified "2019-05-02"^^xsd:date ;
                                          dct:creator [
                                              sdo:name "Nicholas J. Car" ;
                                              sdo:identifier <http://orcid.org/0000-0002-8742-7730> ;
                                          ] ;
                                          rdfs:label "GSQ Borehole Profile" ;
                                          rdfs:comment """The Geological Survey of Queensland's profile of several specifications to characterise a borehole.

This profile contains alignments to specifications that it does not directly profile but is informed by, such as GeoSciML."""@en ;
                                          dct:publisher [
                                            sdo:name "Geological Survey of Queensland" ;
                                            sdo:identifier <http://catalogue.linked.data.gov.au/org/gsq> ;
                                          ] ;
                                          dct:created "2019-04-30"^^xsd:date ;
                                          owl:versionInfo "See the GitHub repo https://github.com/geological-survey-of-queensland/gsq-borehole-profile for versioning"@en .


#################################################################
#    Object Properties
#################################################################

###  http://linked.data.gov.au/def/borehole/driller
:driller rdf:type owl:ObjectProperty ;
         rdfs:subPropertyOf prov:wasAttributedTo ;
         rdfs:range prov:Agent ;
         rdfs:comment "An organisation that drilled the borehole."@en ;
         rdfs:label "driller"@en ;
         skos:scopeNote "If the borehole was drilled by multiple organisations, add multiple :driller properties. Different periods of drilling, as indicated by :hadDrillingTime may have the specific driller indicated by qualifying the Agent (driller) / Activity (drilling episode), as per PROV-O's qualifiedAssociation pattern."@en ;
         sdo:domainIncludes :Borehole .


###  http://linked.data.gov.au/def/borehole/hadDrillingMethod
:hadDrillingMethod rdf:type owl:ObjectProperty ;
                   rdfs:subPropertyOf loci:hadGenerationMethod ;
                   rdfs:domain :Borehole ;
                   rdfs:range skos:Concept ;
                   rdfs:comment "The method of drilling used to create this borehole."@en ;
                   rdfs:label "had drilling method" ;
                   skos:scopeNote """Drilling Methods must be selected from the Borehole Drilling Methods vocabulary. If multiple methods were used, multiple :hadDrillingMethod properties should be used.

This method is a sub property of the Loc-I Ontology's had:GenerationMethod which is a property chain axiom for PROV's  prov:wasGeneratedBy / prov:qualifiedAssociation / prov:hadPlan which allows an Entity (the borehole) to indicate the method (a PROV Plan) that was used to instruct the Activity that generated it (here the event of drilling)."""@en .


###  http://linked.data.gov.au/def/borehole/hadDrillingTime
:hadDrillingTime rdf:type owl:ObjectProperty ;
                 rdfs:subPropertyOf time:hasTime ;
                 rdfs:range time:ProperInterval ;
                 rdfs:comment "The time period during which the borehole was drilled."@en ;
                 rdfs:label "had drilling time"@en ;
                 skos:scopeNote "If the borehole was drilled at multiple times, add multiple :hasDrillingTime properties."@en ;
                 sdo:domainIncludes :Borehole .


###  http://linked.data.gov.au/def/borehole/hasCasing
:hasCasing rdf:type owl:ObjectProperty ;
           rdfs:domain :BoreholeInterval ;
           rdfs:range :Casing ;
           rdfs:comment "Casing is a cladding on the inside of the well / bore shaft"@en ;
           rdfs:label "has casing"@en .


###  http://linked.data.gov.au/def/borehole/hasDiameter
:hasDiameter rdf:type owl:ObjectProperty ;
             rdfs:subPropertyOf qudt:hasQuantity ;
             rdfs:range qudt:Quantity ;
             rdfs:comment "The average width of the borehole shaft."@en ;
             rdfs:label "has diameter"@en ;
             sdo:domainIncludes :Borehole ,
                                :BoreholeInterval .


###  http://linked.data.gov.au/def/borehole/hasElevation
:hasElevation rdf:type owl:ObjectProperty ;
              rdfs:range geox:VerticalGeometry ;
              rdfs:comment "The position of a borehole vertically, with reference to the earthe's surface."@en ;
              rdfs:label "has elevation" ;
              sdo:domainIncludes :Borehole .


###  http://linked.data.gov.au/def/borehole/hasInclination
:hasInclination rdf:type owl:ObjectProperty ;
                rdfs:domain :Borehole ;
                rdfs:range skos:Concept ;
                rdfs:comment "The angle to the vertical of the borehole main shaft."@en ;
                rdfs:label "has inclination" ;
                skos:scopeNote "Inclinations must be selected from the Borehole Inclination vocabulary. If the borehole shaft has multiple angles, multiple :hasInclination properties should be used."@en .


###  http://linked.data.gov.au/def/borehole/hasPurpose
:hasPurpose rdf:type owl:ObjectProperty ;
            rdfs:domain :Borehole ;
            rdfs:range skos:Concept ;
            rdfs:comment "The reason for which this borehole was drilled."@en ;
            rdfs:label "has purpose" ;
            skos:scopeNote "Purposes must be selected from the Borehole Purpose vocabulary. Multiple purposes may be selected. If purposes are time-bound, this should be indicated by assigning the purpose a time:hasTime property."@en .


###  http://linked.data.gov.au/def/borehole/hasStateOrTerritory
:hasStateOrTerritory rdf:type owl:ObjectProperty ;
                     rdfs:range asgs:StateOrTerritory ;
                     rdfs:comment "The Australian State or Territory that this borehole is juristictionally within."@en ;
                     rdfs:label "has state" ;
                     skos:scopeNote "The borehole need bot be spatially within the Australian State or Territory."@en ;
                     sdo:domainIncludes :Borehole .


###  http://linked.data.gov.au/def/borehole/hasStatus
:hasStatus rdf:type owl:ObjectProperty ;
           rdfs:domain :Borehole ;
           rdfs:range skos:Concept ;
           rdfs:comment "The lifecycle stage of the borehole."@en ;
           rdfs:label "has status" ;
           skos:scopeNote "Status must be selected from the Borehole Status vocabulary."@en .


###  http://linked.data.gov.au/def/borehole/hasSurfaceCircumstance
:hasSurfaceCircumstance rdf:type owl:ObjectProperty ;
                        rdfs:domain :Borehole ;
                        rdfs:range skos:Concept ;
                        rdfs:comment "The circumstances of a borehole's entrance." ;
                        rdfs:label "has surface circumstance" ;
                        skos:scopeNote """Surface Circumstances must be selected from the Borehole Surface Circumstance vocabulary.

This property maps to GeoSciML's Borehole Start property.""" .


###  http://linked.data.gov.au/def/borehole/nextBoreholeInterval
:nextBoreholeInterval rdf:type owl:ObjectProperty ;
                      rdfs:domain :BoreholeInterval ;
                      rdfs:range :BoreholeInterval ;
                      rdfs:comment "Indicates the next BoreholeInterval after this one, in the direction away from the Borehole's start"@en ;
                      rdfs:label "next borehole interval"@en .


###  http://linked.data.gov.au/def/borehole/operator
:operator rdf:type owl:ObjectProperty ;
          rdfs:subPropertyOf prov:wasAttributedTo ;
          rdfs:comment "An organisation that maintains/uses/runs the borehole."@en ;
          rdfs:label "operator"@en ;
          skos:scopeNote "If the borehole was/is operated by multiple organisations, add multiple :operator properties. Different periods of operation, may have the specific operator indicated by qualifying the Entity (Borehole) / Agent (operator) relations, as per PROV-O's qualifiedAttribution pattern."@en ;
          sdo:domainIncludes :Borehole .

#################################################################
#    Classes
#################################################################

###  http://linked.data.gov.au/def/borehole/Borehole
:Borehole rdf:type owl:Class ;
          rdfs:subClassOf geo:Feature ,
                          [ rdf:type owl:Restriction ;
                            owl:onProperty :hasStatus ;
                            owl:qualifiedCardinality "1"^^xsd:nonNegativeInteger ;
                            owl:onClass skos:Concept
                          ] ;
          rdfs:comment "A borehole is a narrow shaft bored in the ground. A borehole may be constructed for many different purposes, including the extraction of water, other liquids (such as petroleum) or gases (such as natural gas), as part of a geotechnical investigation, environmental site assessment, mineral exploration, temperature measurement, as a pilot hole for installing piers or underground utilities, for geothermal installations, or for underground storage of unwanted substances, e.g. in carbon capture and storage."@en ;
          rdfs:label "Borehole" .


###  http://linked.data.gov.au/def/borehole/BoreholeInterval
:BoreholeInterval rdf:type owl:Class ;
                  rdfs:subClassOf geo:Feature .


###  http://linked.data.gov.au/def/borehole/Casing
:Casing rdf:type owl:Class ;
        rdfs:subClassOf skos:Concept .


###  http://linked.data.gov.au/def/borehole/Well
:Well rdf:type owl:Class ;
      rdfs:subClassOf :Borehole ;
      rdfs:comment "A Well is a Borehole that is made of multiple Wellbores."@en ;
      rdfs:label "Well"@en .


###  http://linked.data.gov.au/def/borehole/Wellbore
:Wellbore rdf:type owl:Class ;
          rdfs:subClassOf :Borehole ;
          rdfs:comment """Wellbores are a type of Borehole that constitutes part of a Well.

Commonly, Wellbores within a Well share a starting point."""@en ;
          rdfs:label "Wellbore"@en .

###  Generated by the OWL API (version 4.2.8.20170104-2310) https://github.com/owlcs/owlapi
